Clase sobre invariantes

lab2.dfy
@@ -12,19 +12,19 @@ method MaxSumaBackwards(m:nat, s:nat) returns (x:nat, y:nat)
     y:= s-m;
 }
 
-method Main()
-    decreases *;
-{
-    var max, other := MaxSumaBackwards(7,12);
+// method Main()
+//     decreases *;
+// {
+//     var max, other := MaxSumaBackwards(7,12);
     
-    print max;
-    print "\n";
-    print other;
+//     print max;
+//     print "\n";
+//     print other;
 
-    while true 
-        decreases * ;
-    {}
-}
+//     while true 
+//         decreases * ;
+//     {}
+// }
 
 function fact (n:int):int
 	requires n >= 0
@@ -78,73 +78,121 @@ while x <= n
 
 
 // EXERCISE 3
-/*
-method factorial3 (n:int) returns (f:int)
+method factoial3 (n:int) returns (f:int)
 	requires n >= 0
 	ensures f == fact(n)
 {
-var x:int := 0; 
-f := 1;
-while x < n
-	  // invariant 
-	  // invariant 
-	{
-		// assert ;
-	x := x + 1;
-		// assert ;
-	f := f * x;
-	}
+	var x:int := 0; 
+	f := 1;
+	while x < n
+		invariant 0 <= x <= n
+		invariant f == fact(x)
+		{
+		// 	assert 0<=x+1 && f*(x+1) == fact(x+1);
+		// x := x + 1;
+		// 	assert 0<=x<=n && f*x == fact(x);
+		// f := f * x;
+		// 	assert 0<=x<=n && f == fact(x);
+
+			x,f := x+1,f*(x+1);
+		}
 }
-*/
+
 
 // EXERCISE 4
 // Write a method Main that calculates the first 11 factorials and shows the results.
 
-
+method Main ()
+{
+	var i:= 0;
+	var f:= 0;
+	while i < 11
+	invariant 0 <= i <= 11
+	{
+	   f := factoial3(i);
+		print "factoria de ", i, " = ", f , "\n";
+	   i := i + 1;
+	}
+}
 // EXERCISE 5
 // Verify the following recursive method that calculates the number of combinations of m elements out of n,
 // that is the combinatorial number "m over n".
 
 method combinations (m:int, n:int) returns (r:int)
+ 	decreases  m, n
 	requires m >= n >= 0
-	//ensures  r * fact(n) * fact(m-n) == fact(m)  
+	ensures  r == combinations'(m,n)
 {
 if n == 0 || n == m  { r := 1; }
 else { 
      var raux1 := combinations(m-1,n-1);
+	 	//assert  raux1*fact(n-1)*fact(m-n) == fact(m-1); // H.I
 	 var raux2 := combinations(m-1,n);
+	 	// assert raux2*fact(n)*fact(m-n-1) == fact(m-1); // H.I 2
+	 
+	 	// assert (raux1 + raux2)* fact(n) * fact(m-n) == fact(m);
 	 r := raux1 + raux2;
+		// assert  r * fact(n) * fact(m-n) == fact(m);
 	 }
 }
 
+function combinations' (m:int, n:int):int
+ 	decreases  m, n
+	requires m >= n >= 0
+	//ensures  r * fact(n) * fact(m-n) == fact(m)  
+{
+	if n == 0 || n == m 
+	then 1 
+	else combinations'(m-1,n-1) + combinations'(m-1,n)
+}
+
+lemma comb_Lemma(m:int, n:int)
+	requires m>=n>=0
+	ensures combinations'(m,n) * fact(n) * fact(m-n) == fact(m)  
+{}
 // EXERCISE 6
 // Define a function sumSerie(n:int):int such that 
 // (informally) sumSerie(n) == 1 + 3 + ... + (2*n - 1)
 
-
-
+function sumSerie(n:int):int
+	decreases n
+	requires n>=1
+	{
+		if n == 1 then 1 else 2*n-1 + sumSerie(n-1)
+	}
 /*
 Define and prove (even if Dafny proves it automatically)
 the lemma "Lemma_Square" that helps Dafny proving the contract of the following method.
 */
-/*
-lemma Lemma_Square(n:int)
 
-method Square' (a:int) returns (x:int)
-	requires a >= 0
-	ensures x == sumSerie(a)
+lemma Lemma_Square(n:int)
+	requires n >= 1
+	ensures sumSerie(n) == n*n
+{}
+
+method Square (a:int) returns (x:int)
+	requires a >= 1
+	ensures x == a*a
 {
-x := 0;
-var y := 0;
-while  y != a
-		// invariant 
-	{
-    x := x + 2*y + 1;
-	y := y+1;
-	}
-Lemma_Square(?);
+	x := 0;
+	var y := 0;
+	while  y < a
+		invariant 0 <= y <= a
+		invariant y>0 ==> x == sumSerie(y)
+		invariant y == 0 ==> x == 0
+		{
+			//assert y+1 > 0;
+			//assert y>0 ==> x == sumSerie(y);
+			//assert y+1>0 ==> x + 2*(y+1) -1 == x + 2*y + 1 == sumSerie(y+1);
+			y := y+1;
+			//assert y>0 ==> x + 2*y - 1 == sumSerie(y);
+			x := x + 2*y - 1;
+			//assert x == sumSerie(y);
+		}
+	//assert x == sumSerie(a);
+	Lemma_Square(a);
 }
-*/
+
 
 
 
