Main.dfy
@@ -2,5 +2,5 @@ import lab2.dfy as lab2
 
 method Main()
 {
-    var max, other := Ma
+    var max, other := MaxS
 }
